src/ldrfra/PFtoRAThread.v
@@ -250,7 +250,7 @@ Module PFtoRAThread.
     Lemma step_ra_future
           ordr ordw rels1 rels2 e e1 e2
           (WF1: wf_ra rels1 e1)
-          (ORD: Ordering.le Ordering.plain ordw)
+          (ORDC: Ordering.le Ordering.plain ordw)
           (STEP: WThread.step L ordr ordw rels1 rels2 e e1 e2):
       <<WF2_APF: wf_ra rels2 e2>>.
     Proof.
@@ -317,16 +317,11 @@ Module PFtoRAThread.
           (STEP: Thread.reserve_step e1 e2):
       wf_ra rels e2.
     Proof.
-      inv STEP. inv WF1.
-      exploit Thread.step_future; eauto. i. des.
+      inv WF1.
+      hexploit OrdThread.reserve_step_reserve_only; eauto. i. des.
+      hexploit Writes.reserve_step_wf; eauto. i.
+      inv STEP. exploit Thread.step_future; eauto. i. des.
       econs; eauto.
-      - 
-      inv STEP0; inv STEP; inv LOCAL. inv PROMISE. ss.
-      ii. exploit RELS; eauto. i. des. split.
-      - erewrite Memory.add_o; eauto. condtac; ss. des. subst.
-        exploit Memory.add_get0; try exact MEM0. i. des. congr.
-      - erewrite Memory.add_o; eauto. condtac; ss; eauto. des. subst.
-        exploit Memory.add_get0; try exact MEM0. i. des. congr.
     Qed.
 
     Lemma cancel_step_pf_future
@@ -357,14 +352,11 @@ Module PFtoRAThread.
           (STEP: Thread.cancel_step e1 e2):
       wf_ra rels e2.
     Proof.
-      inv STEP. inv WF1.
-      exploit Thread.step_future; eauto. i. des.
+      inv WF1.
+      hexploit OrdThread.cancel_step_reserve_only; eauto. i. des.
+      hexploit Writes.cancel_step_wf; eauto. i.
+      inv STEP. exploit Thread.step_future; eauto. i. des.
       econs; eauto.
-      inv STEP0; inv STEP; inv LOCAL. inv PROMISE. ss.
-      ii. exploit RELS; eauto. i. des. split.
-      - erewrite Memory.remove_o; eauto. condtac; ss.
-      - erewrite Memory.remove_o; eauto. condtac; ss; eauto. des. subst.
-        exploit Memory.remove_get0; try exact MEM0. i. des. congr.
     Qed.
 
     Lemma steps_pf_future
@@ -387,9 +379,10 @@ Module PFtoRAThread.
     Qed.
 
     Lemma steps_ra_future
-          rels1 rels2 e1 e2
+          ordr ordw rels1 rels2 e1 e2
           (WF1: wf_ra rels1 e1)
-          (STEPS: WThread.steps L rels1 rels2 e1 e2):
+          (ORDC: Ordering.le Ordering.plain ordw)
+          (STEPS: WThread.steps L ordr ordw rels1 rels2 e1 e2):
       <<WF2_RA: wf_ra rels2 e2>>.
     Proof.
       induction STEPS; eauto.
@@ -460,277 +453,363 @@ Module PFtoRAThread.
     (* sim_thread *)
 
     Inductive sim_thread (views: Loc.t -> Time.t -> list View.t) (rels: Writes.t)
-                         (e_pf e_j e_ra: Thread.t lang): Prop :=
+                         (e_pf e_j e_apf e_ra: Thread.t lang): Prop :=
     | sim_thread_intro
         (SIM_JOINED: JSim.sim_thread views e_j e_pf)
-        (SIM_RA: APFtoRASim.sim_thread L rels e_ra e_j)
+        (SIM_APF: PFtoAPFSim.sim_thread L rels e_apf e_j)
+        (SIM_RA: APFtoRASim.sim_thread L rels e_ra e_apf)
 
-        (NORMAL_J: APFtoRASim.normal_thread L e_j)
-        (NORMAL_RA: APFtoRASim.normal_thread L e_ra)
-        (STABLE_RA: APFtoRASim.stable_thread L rels e_ra)
+        (NORMAL_APF: Normal.normal_thread L e_apf)
+        (NORMAL_RA: Normal.normal_thread L e_ra)
+        (STABLE_RA: Stable.stable_thread L rels e_ra)
         (CLOSED_VIEWS: closed_views views (Thread.memory e_ra))
         (NORMAL_VIEWS: normal_views views)
         (STABLE_VIEWS: stable_views (Thread.memory e_ra) views)
     .
 
     Lemma sim_thread_step_aux
-          views1 rels1 e1_pf e1_j e1_ra
+          views1 rels1 e1_pf e1_j e1_apf e1_ra
           pf e_pf e2_pf
-          (SIM1: sim_thread views1 rels1 e1_pf e1_j e1_ra)
+          (SIM1: sim_thread views1 rels1 e1_pf e1_j e1_apf e1_ra)
           (JOINED_REL: joined_released views1 (Local.promises (Thread.local e1_j)) (Local.tview (Thread.local e1_j)).(TView.rel))
           (JOINED_MEM: joined_memory views1 (Thread.memory e1_j))
           (JOINED_VIEWS: wf_views views1)
+          (WRITES1_APF: Writes.wf L rels1 (Thread.memory e1_apf))
+          (RESERVE_ONLY1_APF: OrdLocal.reserve_only L (Local.promises (Thread.local e1_apf)))
+          (WRITES1_RA: Writes.wf L rels1 (Thread.memory e1_ra))
+          (RESERVE_ONLY1_RA: OrdLocal.reserve_only L (Local.promises (Thread.local e1_ra)))
           (WF1_PF: Local.wf (Thread.local e1_pf) (Thread.memory e1_pf))
           (SC1_PF: Memory.closed_timemap (Thread.sc e1_pf) (Thread.memory e1_pf))
           (MEM1_PF: Memory.closed (Thread.memory e1_pf))
           (WF1_J: Local.wf (Thread.local e1_j) (Thread.memory e1_j))
           (SC1_J: Memory.closed_timemap (Thread.sc e1_j) (Thread.memory e1_j))
           (MEM1_J: Memory.closed (Thread.memory e1_j))
+          (WF1_APF: Local.wf (Thread.local e1_apf) (Thread.memory e1_apf))
+          (SC1_APF: Memory.closed_timemap (Thread.sc e1_apf) (Thread.memory e1_apf))
+          (MEM1_APF: Memory.closed (Thread.memory e1_apf))
           (WF1_RA: Local.wf (Thread.local e1_ra) (Thread.memory e1_ra))
           (SC1_RA: Memory.closed_timemap (Thread.sc e1_ra) (Thread.memory e1_ra))
           (MEM1_RA: Memory.closed (Thread.memory e1_ra))
           (STEP_PF: Thread.step pf e_pf e1_pf e2_pf)
           (CONS: Local.promise_consistent (Thread.local e2_pf))
           (PROMISE: PF.pf_event L e_pf):
-      exists views2 e_j pf_j e2_j e_ra e2_ra,
-        (<<STEP_J: JThread.step pf_j e_j e1_j e2_j views1 views2>>) /\
-        (<<EVENT_J: JSim.sim_event e_j e_pf>>) /\
-        (<<STEP_RA: OrdThread.step L Ordering.acqrel pf_j e_ra e1_ra e2_ra>>) /\
-        __guard__
-          ((<<SIM2: sim_thread views2 (Writes.append L e_ra rels1) e2_pf e2_j e2_ra>>) /\
-           (<<EVENT_RA: APFtoRASim.sim_event e_ra e_j>>) \/
-           (<<CONS: Local.promise_consistent (Thread.local e1_ra)>>) /\
-           (<<RACE: exists loc to val released ord,
-               ThreadEvent.is_reading e_ra = Some (loc, to, val, released, ord) /\
-               RARaceW.ra_race L rels1 (Local.tview (Thread.local e1_ra)) loc to ord>>)).
+      (exists views2 e_j pf_j e2_j e_apf e2_apf e_ra e2_ra,
+          (<<STEP_J: JThread.step pf_j e_j e1_j e2_j views1 views2>>) /\
+          (<<EVENT_J: JSim.sim_event e_j e_pf>>) /\
+          (<<STEP_APF: OrdThread.step L Ordering.na Ordering.plain pf_j e_apf e1_apf e2_apf>>) /\
+          (<<EVENT_APF: PFtoAPFSim.sim_event e_apf e_j>>) /\
+          (<<STEP_RA: OrdThread.step L Ordering.acqrel Ordering.acqrel pf_j e_ra e1_ra e2_ra>>) /\
+          (<<EVENT_RA: APFtoRASim.sim_event e_ra e_apf>>) /\
+          (<<SIM2: sim_thread views2 (Writes.append L e_ra rels1) e2_pf e2_j e2_apf e2_ra>>)) \/
+      (<<CONS: Local.promise_consistent (Thread.local e1_ra)>>) /\
+      (<<RACE: RARaceW.ra_race L rels1 (Local.tview (Thread.local e1_ra)) (ThreadEvent.get_program_event e_pf)>>).
     Proof.
       hexploit JSim.sim_thread_step; try exact STEP; try eapply SIM1; eauto. i. des.
       destruct (classic (exists loc from to msg kind,
                             e_src = ThreadEvent.promise loc from to msg kind /\ ~ L loc)); cycle 1.
       { (* normal step *)
         inv STEP.
-        hexploit APFtoRASim.thread_step; try exact STEP1; try eapply SIM1; eauto.
-        { i. subst. destruct (L loc) eqn:LOC.
-          - split; ss. inv EVENT. destruct msg; ss. inv MSG.
-            exploit PROMISE; eauto; ss.
-          - exfalso. apply H. esplits; eauto. congr.
+        hexploit PFtoAPFSim.thread_step; try eapply SIM1; eauto.
+        { i. subst. inv EVENT.
+          apply NNPP. ii. apply H. esplits; eauto. ii.
+          apply H0. split; ss.
+          exploit PROMISE; eauto. i. subst. inv MSG. ss.
         }
-        i. unguard. des.
-        - esplits; eauto. left. split; ss.
-          exploit Thread.step_future; try exact STEP_PF; eauto. i. des.
-          exploit Thread.step_future; try eapply STEP0; eauto. i. des.
-          exploit OrdThread.step_future; try exact STEP_SRC; eauto. i. des.
-          econs; eauto.
-          + hexploit future_closed_views; try eapply SIM1; eauto. i.
-            eapply step_closed_views; try eapply SIM1; eauto.
-            * inv WF1. inv TVIEW_CLOSED. apply REL.
-            * i. exploit VIEWSLE; eauto. i. des.
-              inv SIM2. inv MEMORY0.
-              exploit COMPLETE; try exact GET. i. des. inv MSG.
-              inv LOCAL. inv TVIEW. specialize (REL loc). des_ifs.
-              rewrite REL. esplits; eauto.
-          + eapply step_normal_views; try eapply SIM1; eauto.
-            * inv NORMAL2_SRC. inv NORMAL_TVIEW. i. eapply (REL loc).
-            * i. exploit VIEWSLE; eauto. i. des.
-              inv SIM2. inv MEMORY0.
-              exploit COMPLETE; try exact GET. i. des. inv MSG.
-              inv LOCAL. inv TVIEW. specialize (REL loc). des_ifs.
-              rewrite REL. esplits; eauto.
-          + hexploit future_stable_views; try eapply SIM1; eauto. i.
-            eapply step_stable_views; try eapply SIM1; eauto.
-            * inv STABLE2_SRC. inv STABLE_TVIEW. i. eapply (REL loc); eauto.
-            * i. exploit VIEWSLE; eauto. i. des.
-              inv SIM2. inv MEMORY0.
-              exploit COMPLETE; try exact GET. i. des. inv MSG.
-              inv LOCAL. inv TVIEW. specialize (REL loc). des_ifs.
-              rewrite REL. esplits; eauto.
-        - esplits; eauto. right. esplits; eauto.
-          hexploit step_promise_consistent; try exact STEP_PF; try apply SIM1; eauto. i.
-          inv SIM1. inv SIM_JOINED. inv SIM_RA.
-          apply inj_pair2 in H4. subst.
-          apply inj_pair2 in H5. subst. ss.
-          hexploit JSim.sim_local_promise_consistent; try exact LOCAL; eauto. i. des.
-          eapply APFtoRASim.sim_local_promise_consistent; eauto.
+        i. des; cycle 1.
+        { (* race *)
+          right. splits.
+          - eapply APFtoRASim.sim_thread_promise_consistent; try apply SIM1.
+            eapply PFtoAPFSim.sim_thread_promise_consistent; try apply SIM1.
+            inv SIM1. inv SIM_JOINED.
+            apply inj_pair2 in H3, H4. subst. ss.
+            eapply JSim.sim_local_promise_consistent; eauto.
+            hexploit step_promise_consistent; try exact STEP_PF; eauto.
+          - erewrite <- JSim.sim_event_program_event; eauto.
+            erewrite APFtoRASim.sim_thread_ra_race; try apply SIM1; eauto.
+        }
+        hexploit APFtoRASim.thread_step; try exact STEP_SRC; try eapply SIM1; eauto.
+        { i. subst. inv EVENT0. inv EVENT.
+          apply NNPP. ii. apply H. esplits; eauto. ii.
+          apply H0. split; ss.
+          exploit PROMISE; eauto. i. subst. inv MSG. ss.
+        }
+        { inv EVENT0; ss. }
+        { inv EVENT0; ss. }
+        { inv EVENT0; ss. }
+        i. des; cycle 1.
+        { (* race *)
+          right. splits.
+          - eapply APFtoRASim.sim_thread_promise_consistent; try apply SIM1.
+            eapply PFtoAPFSim.sim_thread_promise_consistent; try apply SIM1.
+            inv SIM1. inv SIM_JOINED.
+            apply inj_pair2 in H3, H4. subst. ss.
+            eapply JSim.sim_local_promise_consistent; eauto.
+            hexploit step_promise_consistent; try exact STEP_PF; eauto.
+          - erewrite <- JSim.sim_event_program_event; try eapply EVENT.
+            erewrite <- PFtoAPFSim.sim_event_eq_program_event; try exact EVENT0; eauto.
+        }
+
+        left. unguard. des. esplits; eauto.
+        exploit Thread.step_future; try exact STEP_PF; eauto. i. des.
+        exploit Thread.step_future; try eapply STEP0; eauto. i. des.
+        exploit OrdThread.step_future; try exact STEP_SRC; eauto. i. des.
+        exploit OrdThread.step_future; try exact STEP_SRC0; eauto. i. des.
+        assert (VIEWS: forall loc ts (LOC: ~ L loc) (NEQ: views0 loc ts <> views1 loc ts),
+                   exists from val released,
+                     Memory.get loc ts (Thread.memory e2_src0) = Some (from, Message.concrete val released) /\
+                     views0 loc ts =
+                     (View.join (TView.rel (Local.tview (Thread.local e2_src0)) loc)
+                                (View.singleton_ur loc ts))
+                       :: (all_join_views (View.singleton_ur loc ts) (views1 loc from))).
+        { i. exploit VIEWSLE; eauto. i. des.
+          inv SIM2. inv MEMORY0.
+          unfold Memory.get in GET. rewrite <- EQ in GET; ss.
+          inv SIM0. inv MEMORY0.
+          exploit COMPLETE0; try exact GET. i. des. inv MSG. des_ifs.
+          esplits; eauto.
+          inv LOCAL0. inv TVIEW. specialize (REL loc). des_ifs.
+          rewrite REL. rewrite LOCAL. ss.
+        }
+        econs; eauto.
+        - inv EVENT1; ss.
+        - hexploit future_closed_views; try eapply SIM1; eauto. i.
+          eapply step_closed_views; try eapply SIM1; eauto.
+          inv WF3. inv TVIEW_CLOSED. apply REL.
+        - eapply step_normal_views; try eapply SIM1; eauto.
+          + inv NORMAL2_SRC0. inv NORMAL_TVIEW. i. eapply (REL loc).
+          + i. exploit VIEWS; eauto. i. des. eauto.
+        - hexploit future_stable_views; try eapply SIM1; eauto. i.
+          eapply step_stable_views; try eapply SIM1; eauto.
+          + inv STABLE2_SRC. inv STABLE_TVIEW. i. eapply (REL loc); eauto.
+          + i. exploit VIEWS; eauto. i. des. eauto.
       }
 
       (* promise on ~ L *)
       des. subst. dup STEP. inv STEP0.
       inv STEP1; [|inv STEP0; inv LOCAL]. inv STEP0. ss.
-      hexploit APFtoRASim.promise_step; try exact LOCAL; try eapply SIM1; eauto; try congr. s. i. des.
-      destruct e1_ra. esplits; eauto.
-      { econs.
-        - econs; eauto.
-        - ii. inv PROMISE1. ss.
+      hexploit PFtoAPFSim.promise_step; try exact LOCAL; try eapply SIM1; eauto.
+      { i. destruct msg; ss. exploit PROMISE0; eauto. i. des.
+        inv x; eauto. econs. econs.
+        hexploit Memory.promise_inhabited; try exact PROMISE1; try apply MEM1_APF. i.
+        eapply joined_view_closed; try exact JOINED; eauto.
+        assert (VIEWS1: closed_views views1 mem2_src).
+        { ii. eapply Memory.promise_closed_view; eauto.
+          eapply APFtoRASim.sim_memory_closed_view_src; try eapply SIM1; eauto.
+        }
+        destruct (classic (views0 loc to = views1 loc to)).
+        { rewrite H1. rewrite List.Forall_forall. i. eauto. }
+        exploit VIEWSLE; eauto. i. des. rewrite VIEW.
+        exploit Memory.promise_get0; try exact PROMISE1.
+        { inv PROMISE1; ss. }
+        i. des.
+        exploit Memory.singleton_ur_closed_view; try exact GET_MEM; eauto. i.
+        inv LOCAL. ss. inv SIM1. inv SIM_APF. ss. subst.
+        econs.
+        - eapply Memory.join_closed_view; eauto.
+          eapply Memory.promise_closed_view; try exact PROMISE1.
+          apply WF1_APF.
+        - rewrite List.Forall_forall. i.
+          apply List.in_map_iff in H2. des. subst.
+          eapply Memory.join_closed_view; eauto.
       }
-      left.
-      assert (MSG: forall (val: Const.t) (released: View.t) (MSG: msg = Message.concrete val (Some released)),
-                 Normal.normal_view L released /\ Stable.stable_view L mem2_src released).
-      { i. subst. split.
-        - hexploit (@step_normal_views views1 views0); try eapply SIM1; eauto.
-          { inv SIM1. ss. inv NORMAL_RA. inv NORMAL_TVIEW. i. eapply (REL loc0). }
-          { s. i. exploit VIEWSLE; eauto. i. des.
-            inv MEM2.
-            exploit COMPLETE; try exact GET. i. des. inv MSG.
-            inv LC2. inv TVIEW. specialize (REL loc0). des_ifs.
-            inv STEP_SRC. ss. rewrite REL. esplits; eauto. }
-          i. exploit PROMISE0; eauto. i. des.
-          eapply joined_opt_view_normal_view; eauto.
-        - exploit Local.promise_step_future; try exact STEP_SRC; eauto. s. i. des.
-          hexploit future_closed_views; try eapply SIM1; try exact FUTURE. i.
-          hexploit future_stable_views; try eapply SIM1; try exact FUTURE. i.
-          hexploit (@step_stable_views views1 views0); try exact H1; eauto.
-          { inv SIM1. ss. inv STABLE_RA. ss. inv STABLE_TVIEW.
-            i. hexploit (REL loc0); ss. i.
-            hexploit Stable.future_stable_view; try exact H2; try exact FUTURE; try eapply WF1_RA. i.
-            eapply H3. }
-          { i. exploit VIEWSLE; eauto. i. des.
-            inv MEM2.
-            exploit COMPLETE; try exact GET. i. des. inv MSG.
-            inv LC2. inv TVIEW. specialize (REL loc0). des_ifs.
-            inv STEP_SRC. ss. rewrite REL. esplits; eauto. }
-          i. exploit PROMISE0; eauto. i. des.
-          eapply joined_opt_view_stable_view; eauto.
+      i. des. subst.
+      hexploit APFtoRASim.promise_step; try exact STEP_SRC; try eapply SIM1; eauto; try congr. i. des.
+      destruct e1_apf, e1_ra. ss.
+      left. esplits; eauto.
+      { econs 1; [econs|]; eauto. ii. clarify. }
+      { econs. }
+      { econs 1; [econs|]; eauto. ii. clarify. }
+      { econs. }
+      { assert (VIEWS: forall loc ts (LOC: ~ L loc) (NEQ: views0 loc ts <> views1 loc ts),
+                   exists from val released,
+                     Memory.get loc ts mem2_src0 = Some (from, Message.concrete val released) /\
+                     views0 loc ts =
+                     (View.join (TView.rel (Local.tview lc2_src) loc)
+                                (View.singleton_ur loc ts))
+                       :: (all_join_views (View.singleton_ur loc ts) (views1 loc from))).
+        { i. exploit VIEWSLE; eauto. i. des.
+          inv MEM2.
+          unfold Memory.get in GET. rewrite <- EQ in GET; ss.
+          inv MEM0.
+          exploit COMPLETE0; try exact GET. i. des. inv MSG. des_ifs.
+          esplits; eauto.
+          inv LC2. inv TVIEW. specialize (REL loc0). des_ifs.
+          rewrite REL. ss.
+        }
+        assert (MSG: forall (val: Const.t) (released: View.t) (MSG: msg = Message.concrete val (Some released)),
+                   Normal.normal_view L released /\ Stable.stable_view L mem2_src0 released).
+        { i. subst. split.
+          - hexploit (@step_normal_views views1 views0); try eapply SIM1; eauto.
+            { inv SIM1. ss. inv NORMAL_RA. inv NORMAL_TVIEW. i. eapply (REL loc0). }
+            { s. i. exploit VIEWS; eauto. i. des.
+              inv STEP_SRC0. ss. eauto.
+            }
+            i. exploit PROMISE0; eauto. i. des.
+            eapply joined_opt_view_normal_view; eauto.
+          - exploit Local.promise_step_future; try exact STEP_SRC0; eauto. s. i. des.
+            hexploit future_closed_views; try eapply SIM1; try exact FUTURE. i.
+            hexploit future_stable_views; try eapply SIM1; try exact FUTURE. i.
+            hexploit (@step_stable_views views1 views0); try exact H1; eauto.
+            { inv SIM1. ss. inv STABLE_RA. ss. inv STABLE_TVIEW.
+              i. hexploit (REL loc0); ss. i.
+              hexploit Stable.future_stable_view; try exact H2; try exact FUTURE; try eapply WF1_RA. i.
+              eapply H3.
+            }
+            { i. exploit VIEWS; eauto. i. des.
+              inv STEP_SRC0. ss. eauto.
+            }
+            i. exploit PROMISE0; eauto. i. des.
+            eapply joined_opt_view_stable_view; eauto.
+        }
+
+        hexploit APFtoRASim.sim_memory_stable_tview; try eapply SIM1. s. i.
+        hexploit APFtoRASim.sim_memory_stable_memory; try eapply SIM1. s. i.
+        hexploit Normal.promise_step; try exact STEP_SRC; try eapply SIM1.
+        { i. subst. exploit MSG; eauto. i. des. ss. }
+        i. des.
+        hexploit Normal.promise_step; try exact STEP_SRC0; try eapply SIM1.
+        { i. subst. exploit MSG; eauto. i. des. ss. }
+        i. des.
+        hexploit Stable.promise_step; try exact STEP_SRC0; try eapply SIM1; eauto.
+        { i. subst. exploit MSG; eauto. i. des. ss. }
+        i. des.
+        exploit Local.promise_step_future; try exact STEP_SRC0; eauto. s. i. des.
+        unfold Writes.append. ss.
+        inv SIM1. inv SIM_APF. inv SIM_RA. ss. subst.
+        econs; eauto; ss.
+        - econs; eauto. ss.
+          eapply Stable.future_stable_view; try exact FUTURE; ss.
+          apply STABLE_RA.
+        - hexploit future_closed_views; try eapply SIM1; eauto. i.
+          eapply step_closed_views; try eapply SIM1; eauto.
+          inv WF2. inv TVIEW_CLOSED. apply REL.
+        - eapply step_normal_views; try eapply SIM1; eauto.
+          + inv NORMAL_TVIEW0. i. eapply (REL loc0).
+          + i. exploit VIEWS; eauto. i. des. eauto.
+        - hexploit future_stable_views; try eapply SIM1; eauto. i.
+          eapply step_stable_views; try eapply SIM1; eauto.
+          + inv STABLE_TVIEW2. i. eapply (REL loc0); eauto.
+          + i. exploit VIEWS; eauto. i. des. eauto.
       }
-      hexploit APFtoRASim.sim_memory_stable_tview; try eapply SIM1. s. i.
-      hexploit APFtoRASim.sim_memory_stable_memory; try eapply SIM1. s. i.
-      exploit APFtoRASim.sim_release_writes_wf; try eapply SIM1. s. i. des.
-      hexploit Stable.promise_step; try exact LOCAL; try eapply SIM1; eauto.
-      { i. subst. exploit MSG; eauto. i. des. split; ss.
-        eapply APFtoRASim.sim_memory_stable_view; eauto. }
-      i. des.
-      hexploit Stable.promise_step; try exact STEP_SRC; try eapply SIM1; eauto. i. des.
-      split; try by econs.
-      exploit Thread.step_future; try exact STEP_PF; eauto. i. des.
-      exploit Local.promise_step_future; try exact LOCAL; eauto. s. i. des.
-      exploit Local.promise_step_future; try exact STEP_SRC; eauto. s. i. des.
-      econs; ss; eauto.
-      - inv SIM1. inv SIM_RA. econs; ss; eauto.
-      - unfold Writes.append. ss. econs; ss; eauto.
-        inv SIM1. ss.
-        eapply Stable.future_stable_view; try exact FUTURE0; try eapply SIM; ss.
-        apply STABLE_RA.
-      - hexploit future_closed_views; try eapply SIM1; eauto. i.
-        eapply step_closed_views; try eapply SIM1; eauto.
-        + inv WF1. inv TVIEW_CLOSED. apply REL.
-        + i. exploit VIEWSLE; eauto. i. des.
-          inv MEM2.
-          exploit COMPLETE; try exact GET. i. des. inv MSG0.
-          inv LC2. inv TVIEW. specialize (REL loc0). des_ifs.
-          rewrite REL. esplits; eauto.
-      - eapply step_normal_views; try eapply SIM1; eauto.
-        + inv NORMAL_TVIEW0. i. eapply (REL loc0).
-        + i. exploit VIEWSLE; eauto. i. des.
-          inv MEM2.
-          exploit COMPLETE; try exact GET. i. des. inv MSG0.
-          inv LC2. inv TVIEW. specialize (REL loc0). des_ifs.
-          rewrite REL. esplits; eauto.
-      - hexploit future_stable_views; try eapply SIM1; eauto. i.
-        eapply step_stable_views; try eapply SIM1; eauto.
-        + inv STABLE_TVIEW0. i. eapply (REL loc0); eauto.
-        + i. exploit VIEWSLE; eauto. i. des.
-          inv MEM2.
-          exploit COMPLETE; try exact GET. i. des. inv MSG0.
-          inv LC2. inv TVIEW. specialize (REL loc0). des_ifs.
-          rewrite REL. esplits; eauto.
+    Qed.
+
+    Lemma sim_event_ra_writes_append
+          e_apf e_ra
+          (SIM: APFtoRASim.sim_event e_ra e_apf):
+      forall rels, Writes.append L e_apf rels = Writes.append L e_ra rels.
+    Proof.
+      inv SIM; ss.
     Qed.
 
     Lemma sim_thread_step
-          views1 rels1 e1_pf e1_j e1_ra
+          views1 rels1 e1_pf e1_j e1_apf e1_ra
           pf e_pf e2_pf
-          (SIM1: sim_thread views1 rels1 e1_pf e1_j e1_ra)
+          (SIM1: sim_thread views1 rels1 e1_pf e1_j e1_apf e1_ra)
           (WF1_PF: wf_pf e1_pf)
           (WF1_J: wf_j views1 e1_j)
+          (WF1_APF: wf_ra rels1 e1_apf)
           (WF1_RA: wf_ra rels1 e1_ra)
           (STEP: Thread.step pf e_pf e1_pf e2_pf)
           (PF: PF.pf_event L e_pf)
           (CONS: Local.promise_consistent (Thread.local e2_pf)):
-      (exists views2 rels2 pf_j e_j e2_j e_ra e2_ra,
+      (exists views2 rels2 pf_j e_j e2_j e_apf e2_apf e_ra e2_ra,
           (<<STEP_J: JThread.step pf_j e_j e1_j e2_j views1 views2>>) /\
+          (<<STEP_APF: WThread.step L Ordering.na Ordering.plain rels1 rels2 e_apf e1_apf e2_apf>>) /\
           (<<STEP_RA: WThread.step L Ordering.acqrel Ordering.acqrel rels1 rels2 e_ra e1_ra e2_ra>>) /\
           (<<EVENT_J: JSim.sim_event e_j e_pf>>) /\
-          (<<EVENT_RA: APFtoRASim.sim_event e_ra e_j>>) /\
-          (<<SIM2: sim_thread views2 rels2 e2_pf e2_j e2_ra>>)) \/
-      (exists rels2 e_ra e2_ra loc to val released ord,
-          (<<CONS_RA: Local.promise_consistent (Thread.local e1_ra)>>) /\
-          (<<STEP_RA: WThread.step L Ordering.acqrel Ordering.acqrel rels1 rels2 e_ra e1_ra e2_ra>>) /\
-          (<<READ: ThreadEvent.is_reading e_ra = Some (loc, to, val, released, ord)>>) /\
-          (<<RACE: RARaceW.ra_race L rels1 (Local.tview (Thread.local e1_ra)) loc to ord>>)).
+          (<<EVENT_APF: PFtoAPFSim.sim_event e_apf e_j>>) /\
+          (<<EVENT_RA: APFtoRASim.sim_event e_ra e_apf>>) /\
+          (<<SIM2: sim_thread views2 rels2 e2_pf e2_j e2_apf e2_ra>>)) \/
+      (exists e st2,
+          (<<CONS: Local.promise_consistent (Thread.local e1_ra)>>) /\
+          (<<STEP: lang.(Language.step) e e1_ra.(Thread.state) st2>>) /\
+          (<<RACE: RARaceW.ra_race L rels1 (Local.tview (Thread.local e1_ra)) e>>)).
     Proof.
-      exploit sim_thread_step_aux; eauto; try apply WF1_PF; try apply WF1_J; try apply WF1_RA.
-      i. unguard. des.
-      - left. esplits; eauto.
-        + econs 1. eauto.
-      - right. esplits; eauto. econs; eauto.
+      exploit sim_thread_step_aux; eauto; try apply WF1_PF; try apply WF1_J; try apply WF1_APF; try apply WF1_RA.
+      i. des.
+      { left. esplits; eauto.
+        - erewrite <- sim_event_ra_writes_append; eauto.
+          econs. eauto.
+        - econs. eauto.
+      }
+      right.
+      inv SIM1. inv SIM_JOINED.
+      apply inj_pair2 in H2, H3. subst.
+      destruct e1_apf, e1_ra.
+      inv SIM_APF. inv SIM_RA. ss. subst.
+      inv STEP.
+      { inv STEP0. unfold RARaceW.ra_race in *. des; ss. }
+      inv STEP0. esplits; eauto.
     Qed.
 
     Lemma sim_thread_opt_step
-          views1 rels1 e1_pf e1_j e1_ra
+          views1 rels1 e1_pf e1_j e1_apf e1_ra
           e_pf e2_pf
-          (SIM1: sim_thread views1 rels1 e1_pf e1_j e1_ra)
+          (SIM1: sim_thread views1 rels1 e1_pf e1_j e1_apf e1_ra)
           (WF1_PF: wf_pf e1_pf)
           (WF1_J: wf_j views1 e1_j)
+          (WF1_APF: wf_ra rels1 e1_apf)
           (WF1_RA: wf_ra rels1 e1_ra)
           (STEP: Thread.opt_step e_pf e1_pf e2_pf)
           (PF: PF.pf_event L e_pf)
           (CONS: Local.promise_consistent (Thread.local e2_pf)):
-      (exists views2 rels2 e_j e2_j e_ra e2_ra,
+      (exists views2 rels2 e_j e2_j e_apf e2_apf e_ra e2_ra,
           (<<STEP_J: JThread.opt_step e_j e1_j e2_j views1 views2>>) /\
-          (<<STEP_RA: WThread.opt_step L rels1 rels2 e_ra e1_ra e2_ra>>) /\
+          (<<STEP_APF: WThread.opt_step L Ordering.na Ordering.plain rels1 rels2 e_apf e1_apf e2_apf>>) /\
+          (<<STEP_RA: WThread.opt_step L Ordering.acqrel Ordering.acqrel rels1 rels2 e_ra e1_ra e2_ra>>) /\
           (<<EVENT_J: JSim.sim_event e_j e_pf>>) /\
-          (<<EVENT_RA: APFtoRASim.sim_event e_ra e_j>>) /\
-          (<<SIM2: sim_thread views2 rels2 e2_pf e2_j e2_ra>>)) \/
-      (exists rels2 e_ra e2_ra loc to val released ord,
-          (<<CONS_RA: Local.promise_consistent (Thread.local e1_ra)>>) /\
-          (<<STEP_RA: WThread.step L Ordering.acqrel Ordering.acqrel rels1 rels2 e_ra e1_ra e2_ra>>) /\
-          (<<READ: ThreadEvent.is_reading e_ra = Some (loc, to, val, released, ord)>>) /\
-          (<<RACE: RARaceW.ra_race L rels1 (Local.tview (Thread.local e1_ra)) loc to ord>>)).
+          (<<EVENT_APF: PFtoAPFSim.sim_event e_apf e_j>>) /\
+          (<<EVENT_RA: APFtoRASim.sim_event e_ra e_apf>>) /\
+          (<<SIM2: sim_thread views2 rels2 e2_pf e2_j e2_apf e2_ra>>)) \/
+      (exists e st2,
+          (<<CONS: Local.promise_consistent (Thread.local e1_ra)>>) /\
+          (<<STEP: lang.(Language.step) e e1_ra.(Thread.state) st2>>) /\
+          (<<RACE: RARaceW.ra_race L rels1 (Local.tview (Thread.local e1_ra)) e>>)).
     Proof.
       inv STEP.
-      - left. esplits; eauto; try econs 1. econs.
+      - left. esplits; eauto; try econs 1; econs.
       - exploit sim_thread_step; eauto. i. des.
-        + left. esplits.
-          * econs 2; eauto.
-          * econs 2; eauto.
-          * ss.
-          * ss.
-          * ss.
-        + right. esplits; eauto.
+        + left. esplits; (try by econs 2; eauto); ss.
+        + right. eauto.
     Qed.
 
     Lemma sim_thread_steps
-          views1 rels1 e1_pf e1_j e1_ra
+          views1 rels1 e1_pf e1_j e1_apf e1_ra
           tr e2_pf
-          (SIM1: sim_thread views1 rels1 e1_pf e1_j e1_ra)
+          (SIM1: sim_thread views1 rels1 e1_pf e1_j e1_apf e1_ra)
           (WF1_PF: wf_pf e1_pf)
           (WF1_J: wf_j views1 e1_j)
+          (WF1_APF: wf_ra rels1 e1_apf)
           (WF1_RA: wf_ra rels1 e1_ra)
           (STEPS: Trace.steps tr e1_pf e2_pf)
           (SILENT: List.Forall (fun the => ThreadEvent.get_machine_event (snd the) = MachineEvent.silent) tr)
           (PF: List.Forall (compose (PF.pf_event L) snd) tr)
           (CONS: Local.promise_consistent (Thread.local e2_pf)):
-      (exists views2 rels2 e2_j e2_ra,
+      (exists views2 rels2 e2_j e2_apf e2_ra,
           (<<STEPS_J: JThread.rtc_tau e1_j e2_j views1 views2>>) /\
-          (<<STEPS_RA: WThread.tau_steps L rels1 rels2 e1_ra e2_ra>>) /\
-          (<<SIM2: sim_thread views2 rels2 e2_pf e2_j e2_ra>>)) \/
-      (exists rels2 rels3 e_ra e2_ra e3_ra loc to val released ord,
-          (<<STEPS_RA: WThread.tau_steps L rels1 rels2 e1_ra e2_ra>>) /\
+          (<<STEPS_APF: WThread.tau_steps L Ordering.na Ordering.plain rels1 rels2 e1_apf e2_apf>>) /\
+          (<<STEPS_RA: WThread.tau_steps L Ordering.acqrel Ordering.acqrel rels1 rels2 e1_ra e2_ra>>) /\
+          (<<SIM2: sim_thread views2 rels2 e2_pf e2_j e2_apf e2_ra>>)) \/
+      (exists rels2 e2_ra e st3,
+          (<<STEPS_RA: WThread.tau_steps L Ordering.acqrel Ordering.acqrel rels1 rels2 e1_ra e2_ra>>) /\
           (<<CONS_RA: Local.promise_consistent (Thread.local e2_ra)>>) /\
-          (<<STEP_RA: WThread.step L Ordering.acqrel Ordering.acqrel rels2 rels3 e_ra e2_ra e3_ra>>) /\
-          (<<READ: ThreadEvent.is_reading e_ra = Some (loc, to, val, released, ord)>>) /\
-          (<<RACE: RARaceW.ra_race L rels2 (Local.tview (Thread.local e2_ra)) loc to ord>>)).
+          (<<STEP_RA: lang.(Language.step) e e2_ra.(Thread.state) st3>>) /\
+          (<<RACE: RARaceW.ra_race L rels2 (Local.tview (Thread.local e2_ra)) e>>)).
     Proof.
-      revert views1 rels1 e1_j e1_ra SIM1 WF1_PF WF1_J WF1_RA SILENT PF CONS.
+      revert views1 rels1 e1_j e1_apf e1_ra SIM1 WF1_PF WF1_J WF1_APF WF1_RA SILENT PF CONS.
       induction STEPS; i; ss.
-      { left. esplits; eauto. econs 1; eauto. }
+      { left. esplits; eauto; econs 1; eauto. }
       subst. exploit sim_thread_step; try exact SIM1; eauto.
       { ii. inv PF. exploit H1; ss; eauto. }
       { exploit Thread.step_future; try exact STEP; try apply WF1_PF. i. des.
         eapply rtc_tau_step_promise_consistent; try eapply Trace.silent_steps_tau_steps; eauto.
-        inv SILENT. ss. }
-      i. unguard. des.
+        inv SILENT. ss.
+      }
+      i. des.
       - exploit step_pf_future; eauto. i. des.
         exploit step_j_future; eauto. i. des.
-        exploit step_ra_future; eauto. i. des.
+        exploit step_ra_future; try exact WF1_APF; eauto; ss. i. des.
+        exploit step_ra_future; try exact WF1_RA; eauto; ss. i. des.
         exploit IHSTEPS; eauto.
         { inv SILENT. ss. }
         { inv PF. ss. }
@@ -739,124 +818,148 @@ Module PFtoRAThread.
           * econs 2; [eauto|..]; eauto.
             inv SILENT. ss. inv EVENT_J; ss.
           * econs 2; [eauto|..]; eauto.
-            inv SILENT. ss. inv EVENT_J; inv EVENT_RA; ss.
+            inv SILENT. ss. inv EVENT_J; inv EVENT_APF; ss.
+          * econs 2; [eauto|..]; eauto.
+            inv SILENT. ss. inv EVENT_J; inv EVENT_APF; inv EVENT_RA; ss.
         + right. esplits; eauto.
           econs 2; [eauto|..]; eauto.
-          inv SILENT. ss. inv EVENT_J; inv EVENT_RA; ss.
+          inv SILENT. ss. inv EVENT_J; inv EVENT_APF; inv EVENT_RA; ss.
       - right. esplits; eauto. econs 1.
     Qed.
 
     Lemma sim_thread_reserve_step
-          views1 rels1 e1_pf e1_j e1_ra
+          views1 rels1 e1_pf e1_j e1_apf e1_ra
           e2_pf
-          (SIM1: sim_thread views1 rels1 e1_pf e1_j e1_ra)
+          (SIM1: sim_thread views1 rels1 e1_pf e1_j e1_apf e1_ra)
           (WF1_PF: wf_pf e1_pf)
           (WF1_J: wf_j views1 e1_j)
+          (WF1_APF: wf_ra rels1 e1_apf)
           (WF1_RA: wf_ra rels1 e1_ra)
           (STEP: Thread.reserve_step e1_pf e2_pf)
           (CONS: Local.promise_consistent (Thread.local e2_pf)):
-      exists e2_j e2_ra,
+      exists e2_j e2_apf e2_ra,
         (<<STEP_J: JThread.reserve_step views1 e1_j e2_j>>) /\
+        (<<STEP_APF: Thread.reserve_step e1_apf e2_apf>>) /\
         (<<STEP_RA: Thread.reserve_step e1_ra e2_ra>>) /\
-        (<<SIM2: sim_thread views1 rels1 e2_pf e2_j e2_ra>>).
+        (<<SIM2: sim_thread views1 rels1 e2_pf e2_j e2_apf e2_ra>>).
     Proof.
       exploit JSim.sim_thread_reserve_step;
         try eapply SIM1; try eapply WF1_PF; try eapply WF1_J; eauto.
       i. des. inv STEP0. inv STEP1.
-      exploit APFtoRASim.reserve_step;
-        try eapply SIM1; try eapply WF1_J; try eapply WF1_RA.
+      exploit PFtoAPFSim.reserve_step;
+        try eapply SIM1; try eapply WF1_J; try eapply WF1_APF.
       { econs; eauto. }
+      i. des.
+      exploit APFtoRASim.reserve_step;
+        try eapply SIM1; try eapply WF1_APF; try eapply WF1_RA; eauto.
       i. des.
       esplits; eauto.
       exploit Thread.rtc_reserve_step_future; [econs 2|..];
-        try eapply STEP_SRC; try eapply WF1_RA; eauto. i. des.
+        try eapply STEP_SRC; try eapply WF1_APF; eauto. i. des.
+      exploit Thread.rtc_reserve_step_future; [econs 2|..];
+        try eapply STEP_SRC0; try eapply WF1_RA; eauto. i. des.
       hexploit future_closed_views; try eapply SIM1; eauto. i.
       hexploit future_stable_views; try eapply SIM1; eauto. i.
       econs; eauto. apply SIM1.
     Qed.
 
     Lemma sim_thread_reserve_steps
-          views1 rels1 e1_pf e1_j e1_ra
+          views1 rels1 e1_pf e1_j e1_apf e1_ra
           e2_pf
-          (SIM1: sim_thread views1 rels1 e1_pf e1_j e1_ra)
+          (SIM1: sim_thread views1 rels1 e1_pf e1_j e1_apf e1_ra)
           (WF1_PF: wf_pf e1_pf)
           (WF1_J: wf_j views1 e1_j)
+          (WF1_APF: wf_ra rels1 e1_apf)
           (WF1_RA: wf_ra rels1 e1_ra)
           (STEP: rtc (@Thread.reserve_step _) e1_pf e2_pf)
           (CONS: Local.promise_consistent (Thread.local e2_pf)):
-      exists e2_j e2_ra,
+      exists e2_j e2_apf e2_ra,
         (<<STEP_J: rtc (@JThread.reserve_step views1 _) e1_j e2_j>>) /\
+        (<<STEP_APF: rtc (@Thread.reserve_step _) e1_apf e2_apf>>) /\
         (<<STEP_RA: rtc (@Thread.reserve_step _) e1_ra e2_ra>>) /\
-        (<<SIM2: sim_thread views1 rels1 e2_pf e2_j e2_ra>>).
+        (<<SIM2: sim_thread views1 rels1 e2_pf e2_j e2_apf e2_ra>>).
     Proof.
-      revert e1_j e1_ra SIM1 WF1_PF WF1_J WF1_RA.
+      revert e1_j e1_apf e1_ra SIM1 WF1_PF WF1_J WF1_APF WF1_RA.
       induction STEP; i; [esplits; eauto|].
       exploit sim_thread_reserve_step; eauto.
       { eapply rtc_reserve_step_promise_consistent; eauto. }
       i. des.
       exploit reserve_step_pf_future; eauto. i.
       exploit reserve_step_j_future; eauto. i.
-      exploit reserve_step_ra_future; eauto. i.
+      exploit reserve_step_ra_future; try exact STEP_APF; eauto. i.
+      exploit reserve_step_ra_future; try exact STEP_RA; eauto. i.
       exploit IHSTEP; eauto. i. des.
       esplits.
+      - econs 2; eauto.
       - econs 2; eauto.
       - econs 2; eauto.
       - ss.
     Qed.
 
     Lemma sim_thread_cancel_step
-          views1 rels1 e1_pf e1_j e1_ra
+          views1 rels1 e1_pf e1_j e1_apf e1_ra
           e2_pf
-          (SIM1: sim_thread views1 rels1 e1_pf e1_j e1_ra)
+          (SIM1: sim_thread views1 rels1 e1_pf e1_j e1_apf e1_ra)
           (WF1_PF: wf_pf e1_pf)
           (WF1_J: wf_j views1 e1_j)
+          (WF1_APF: wf_ra rels1 e1_apf)
           (WF1_RA: wf_ra rels1 e1_ra)
           (STEP: Thread.cancel_step e1_pf e2_pf)
           (CONS: Local.promise_consistent (Thread.local e2_pf)):
-      exists e2_j e2_ra,
+      exists e2_j e2_apf e2_ra,
         (<<STEP_J: JThread.cancel_step views1 e1_j e2_j>>) /\
+        (<<STEP_APF: Thread.cancel_step e1_apf e2_apf>>) /\
         (<<STEP_RA: Thread.cancel_step e1_ra e2_ra>>) /\
-        (<<SIM2: sim_thread views1 rels1 e2_pf e2_j e2_ra>>).
+        (<<SIM2: sim_thread views1 rels1 e2_pf e2_j e2_apf e2_ra>>).
     Proof.
       exploit JSim.sim_thread_cancel_step;
         try eapply SIM1; try eapply WF1_PF; try eapply WF1_J; eauto.
       i. des. inv STEP0. inv STEP1.
-      exploit APFtoRASim.cancel_step;
-        try eapply SIM1; try eapply WF1_J; try eapply WF1_RA.
+      exploit PFtoAPFSim.cancel_step;
+        try eapply SIM1; try eapply WF1_J; try eapply WF1_APF.
       { econs; eauto. }
+      i. des.
+      exploit APFtoRASim.cancel_step;
+        try eapply SIM1; try eapply WF1_APF; try eapply WF1_RA; eauto.
       i. des.
       esplits; eauto.
       exploit Thread.rtc_cancel_step_future; [econs 2|..];
-        try eapply STEP_SRC; try eapply WF1_RA; eauto. i. des.
+        try eapply STEP_SRC; try eapply WF1_APF; eauto. i. des.
+      exploit Thread.rtc_cancel_step_future; [econs 2|..];
+        try eapply STEP_SRC0; try eapply WF1_RA; eauto. i. des.
       hexploit future_closed_views; try eapply SIM1; eauto. i.
       hexploit future_stable_views; try eapply SIM1; eauto. i.
       econs; eauto. apply SIM1.
     Qed.
 
     Lemma sim_thread_cancel_steps
-          views1 rels1 e1_pf e1_j e1_ra
+          views1 rels1 e1_pf e1_j e1_apf e1_ra
           e2_pf
-          (SIM1: sim_thread views1 rels1 e1_pf e1_j e1_ra)
+          (SIM1: sim_thread views1 rels1 e1_pf e1_j e1_apf e1_ra)
           (WF1_PF: wf_pf e1_pf)
           (WF1_J: wf_j views1 e1_j)
+          (WF1_APF: wf_ra rels1 e1_apf)
           (WF1_RA: wf_ra rels1 e1_ra)
           (STEP: rtc (@Thread.cancel_step _) e1_pf e2_pf)
           (CONS: Local.promise_consistent (Thread.local e2_pf)):
-      exists e2_j e2_ra,
+      exists e2_j e2_apf e2_ra,
         (<<STEP_J: rtc (@JThread.cancel_step views1 _) e1_j e2_j>>) /\
+        (<<STEP_APF: rtc (@Thread.cancel_step _) e1_apf e2_apf>>) /\
         (<<STEP_RA: rtc (@Thread.cancel_step _) e1_ra e2_ra>>) /\
-        (<<SIM2: sim_thread views1 rels1 e2_pf e2_j e2_ra>>).
+        (<<SIM2: sim_thread views1 rels1 e2_pf e2_j e2_apf e2_ra>>).
     Proof.
-      revert e1_j e1_ra SIM1 WF1_PF WF1_J WF1_RA.
+      revert e1_j e1_apf e1_ra SIM1 WF1_PF WF1_J WF1_APF WF1_RA.
       induction STEP; i; [esplits; eauto|].
       exploit sim_thread_cancel_step; eauto.
       { eapply rtc_cancel_step_promise_consistent; eauto. }
       i. des.
       exploit cancel_step_pf_future; eauto. i.
       exploit cancel_step_j_future; eauto. i.
-      exploit cancel_step_ra_future; eauto. i.
+      exploit cancel_step_ra_future; try exact STEP_APF; eauto. i.
+      exploit cancel_step_ra_future; try exact STEP_RA; eauto. i.
       exploit IHSTEP; eauto. i. des.
       esplits.
+      - econs 2; eauto.
       - econs 2; eauto.
       - econs 2; eauto.
       - ss.
@@ -866,92 +969,87 @@ Module PFtoRAThread.
     (* consistency *)
 
     Lemma cap_wf_pf
-          e sc mem
+          e mem
           (WF: wf_pf e)
-          (CAP: Memory.cap (Thread.memory e) mem)
-          (SC: Memory.max_concrete_timemap mem sc):
-      wf_pf (Thread.mk lang (Thread.state e) (Thread.local e) sc mem).
+          (CAP: Memory.cap (Thread.memory e) mem):
+      wf_pf (Thread.mk lang (Thread.state e) (Thread.local e) (Thread.sc e) mem).
     Proof.
       inv WF.
       exploit Local.cap_wf; eauto. i.
       exploit Memory.cap_closed; eauto. i.
-      hexploit Memory.max_concrete_timemap_closed; eauto.
+      hexploit Memory.cap_closed_timemap; eauto.
     Qed.
 
     Lemma cap_wf_j
-          views e sc mem
+          views e mem
           (WF: wf_j views e)
-          (CAP: Memory.cap (Thread.memory e) mem)
-          (SC: Memory.max_concrete_timemap mem sc):
-      wf_j views (Thread.mk lang (Thread.state e) (Thread.local e) sc mem).
+          (CAP: Memory.cap (Thread.memory e) mem):
+      wf_j views (Thread.mk lang (Thread.state e) (Thread.local e) (Thread.sc e) mem).
     Proof.
       inv WF.
       exploit Local.cap_wf; eauto. i.
       exploit Memory.cap_closed; eauto. i.
-      hexploit Memory.max_concrete_timemap_closed; eauto. i.
+      hexploit Memory.cap_closed_timemap; eauto.
       exploit JSim.joined_memory_cap; eauto.
     Qed.
 
     Lemma cap_wf_ra
-          rels e sc mem
+          rels e mem
           (WF: wf_ra rels e)
-          (CAP: Memory.cap (Thread.memory e) mem)
-          (SC: Memory.max_concrete_timemap mem sc):
-      wf_ra rels (Thread.mk lang (Thread.state e) (Thread.local e) sc mem).
+          (CAP: Memory.cap (Thread.memory e) mem):
+      wf_ra rels (Thread.mk lang (Thread.state e) (Thread.local e) (Thread.sc e) mem).
     Proof.
       inv WF.
       exploit Local.cap_wf; eauto. i.
       exploit Memory.cap_closed; eauto. i.
-      hexploit Memory.max_concrete_timemap_closed; eauto. i.
+      hexploit Memory.cap_closed_timemap; eauto. i.
       econs; ss.
-      ii. exploit RELS; eauto. i. des.
-      inv CAP. exploit SOUND; eauto.
+      eapply Writes.cap_wf; try exact CAP; eauto.
     Qed.
 
     Lemma sim_thread_cap
-          views rels e_pf e_j e_ra
-          sc_pf mem_pf sc_j mem_j sc_ra mem_ra
-          (SIM: sim_thread views rels e_pf e_j e_ra)
+          views rels e_pf e_j e_apf e_ra
+          mem_pf mem_j mem_apf mem_ra
+          (SIM: sim_thread views rels e_pf e_j e_apf e_ra)
           (WF_PF: wf_pf e_pf)
           (WF_J: wf_j views e_j)
+          (WF_APF: wf_ra rels e_apf)
           (WF_RA: wf_ra rels e_ra)
           (CAP_PF: Memory.cap (Thread.memory e_pf) mem_pf)
-          (SC_PF: Memory.max_concrete_timemap mem_pf sc_pf)
           (CAP_J: Memory.cap (Thread.memory e_j) mem_j)
-          (SC_J: Memory.max_concrete_timemap mem_j sc_j)
-          (CAP_RA: Memory.cap (Thread.memory e_ra) mem_ra)
-          (SC_RA: Memory.max_concrete_timemap mem_ra sc_ra):
+          (CAP_APF: Memory.cap (Thread.memory e_apf) mem_apf)
+          (CAP_RA: Memory.cap (Thread.memory e_ra) mem_ra):
       (<<SIM_CAP: sim_thread views rels
-                             (Thread.mk lang (Thread.state e_pf) (Thread.local e_pf) sc_pf mem_pf)
-                             (Thread.mk lang (Thread.state e_j) (Thread.local e_j) sc_j mem_j)
-                             (Thread.mk lang (Thread.state e_ra) (Thread.local e_ra) sc_ra mem_ra)>>) /\
-      (<<WF_PF_CAP: wf_pf (Thread.mk lang (Thread.state e_pf) (Thread.local e_pf) sc_pf mem_pf)>>) /\
-      (<<WF_J_CAP: wf_j views (Thread.mk lang (Thread.state e_j) (Thread.local e_j) sc_j mem_j)>>) /\
-      (<<WF_RA_CAP: wf_ra rels (Thread.mk lang (Thread.state e_ra) (Thread.local e_ra) sc_ra mem_ra)>>).
+                             (Thread.mk lang (Thread.state e_pf) (Thread.local e_pf) (Thread.sc e_pf) mem_pf)
+                             (Thread.mk lang (Thread.state e_j) (Thread.local e_j) (Thread.sc e_j) mem_j)
+                             (Thread.mk lang (Thread.state e_apf) (Thread.local e_apf) (Thread.sc e_apf) mem_apf)
+                             (Thread.mk lang (Thread.state e_ra) (Thread.local e_ra) (Thread.sc e_ra) mem_ra)>>) /\
+      (<<WF_PF_CAP: wf_pf (Thread.mk lang (Thread.state e_pf) (Thread.local e_pf) (Thread.sc e_pf) mem_pf)>>) /\
+      (<<WF_J_CAP: wf_j views (Thread.mk lang (Thread.state e_j) (Thread.local e_j) (Thread.sc e_j) mem_j)>>) /\
+      (<<WF_APF_CAP: wf_ra rels (Thread.mk lang (Thread.state e_apf) (Thread.local e_apf) (Thread.sc e_apf) mem_apf)>>) /\
+      (<<WF_RA_CAP: wf_ra rels (Thread.mk lang (Thread.state e_ra) (Thread.local e_ra) (Thread.sc e_ra) mem_ra)>>).
     Proof.
       exploit cap_wf_pf; eauto. i.
       exploit cap_wf_j; eauto. i.
-      exploit cap_wf_ra; eauto. i.
+      exploit cap_wf_ra; try exact WF_APF; eauto. i.
+      exploit cap_wf_ra; try exact WF_RA; eauto. i.
       splits; ss.
       inv SIM. econs; ss.
       - inv WF_PF. inv WF_J. inv x0. inv x1. inv SIM_JOINED.
         apply inj_pair2 in H2. apply inj_pair2 in H3. subst. ss.
         econs; eauto.
-        + eapply SimMemory.sim_memory_cap; eauto.
-        + eapply SimMemory.sim_memory_cap in MEM; eauto.
-          eapply SimMemory.sim_memory_max_concrete_timemap in MEM; eauto.
-          subst. refl.
+        eapply SimMemory.sim_memory_cap; eauto.
+      - inv SIM_APF. econs; ss.
+        eapply PFtoAPFSim.sim_memory_cap; eauto; try apply WF_J; try apply WF_APF.
       - inv SIM_RA. econs; ss.
-        + exploit APFtoRASim.sim_memory_cap; eauto; try apply WF_J; try apply WF_RA. i.
-          eapply APFtoRASim.sim_memory_max_concrete_timemap; eauto.
-        + eapply APFtoRASim.sim_memory_cap; eauto; try apply WF_J; try apply WF_RA.
-      - inv NORMAL_J. econs; ss.
-        eapply Stable.cap_normal_memory; eauto. apply WF_J.
+        eapply APFtoRASim.sim_memory_cap; eauto; try apply WF_APF; try apply WF_RA.
+      - inv NORMAL_APF. econs; ss.
+        eapply Stable.cap_normal_memory; eauto. apply WF_APF.
       - inv NORMAL_RA. econs; ss.
         eapply Stable.cap_normal_memory; eauto. apply WF_RA.
       - inv WF_RA. inv STABLE_RA. econs; ss.
         + eapply Stable.cap_stable_tview; eauto.
-        + eapply Stable.max_concrete_timemap_stable; eauto; try apply x2.
+        + eapply Stable.cap_stable_timemap; eauto.
         + eapply Stable.cap_stable_memory; eauto.
       - ii. eapply Memory.cap_closed_view; eauto.
       - ii. exploit Memory.cap_inv; try exact CAP_RA; eauto; try apply WF_RA. i. des; ss.
@@ -974,110 +1072,133 @@ Module PFtoRAThread.
     Qed.
 
     Lemma local_map_ra_race
-          lc1 lc2 rels loc to ordr
+          lc1 lc2 rels e
           (LOCAL: local_map ident_map lc1 lc2)
-          (RARACE: RARaceW.ra_race L rels (Local.tview lc1) loc to ordr):
-      RARaceW.ra_race L rels (Local.tview lc2) loc to ordr.
+          (RARACE: RARaceW.ra_race L rels (Local.tview lc1) e):
+      RARaceW.ra_race L rels (Local.tview lc2) e.
     Proof.
       destruct lc1, lc2. ss. inv LOCAL. ss.
-      unfold RARaceW.ra_race in *. des; splits; eauto.
-      - eapply TimeFacts.le_lt_lt; eauto.
+      unfold RARaceW.ra_race, RARaceW.wr_race, RARaceW.ww_race in *. des.
+      - left. esplits; eauto.
+        eapply TimeFacts.le_lt_lt; eauto.
         inv TVIEW. inv map_cur. rewrite map_rlx. apply TVIEWLE.
-      - eapply TimeFacts.le_lt_lt; eauto.
+      - left. esplits; eauto.
+        eapply TimeFacts.le_lt_lt; eauto.
+        inv TVIEW. inv map_cur. rewrite map_rlx. apply TVIEWLE.
+      - right. esplits; eauto.
+        eapply TimeFacts.le_lt_lt; eauto.
+        inv TVIEW. inv map_cur. rewrite map_rlx. apply TVIEWLE.
+      - right. esplits; eauto.
+        eapply TimeFacts.le_lt_lt; eauto.
         inv TVIEW. inv map_cur. rewrite map_rlx. apply TVIEWLE.
     Qed.
 
     Lemma sim_thread_consistent
-          views1 rels1 e1_pf e1_j e1_ra
-          (SIM1: sim_thread views1 rels1 e1_pf e1_j e1_ra)
+          views1 rels1 e1_pf e1_j e1_apf e1_ra
+          (SIM1: sim_thread views1 rels1 e1_pf e1_j e1_apf e1_ra)
           (WF1_PF: wf_pf e1_pf)
           (WF1_J: wf_j views1 e1_j)
+          (WF1_APF: wf_ra rels1 e1_apf)
           (WF1_RA: wf_ra rels1 e1_ra)
           (CONSISTENT: PF.pf_consistent L e1_pf):
       (<<CONSISTENT_J: JThread.consistent e1_j views1>>) /\
-      ((<<CONSISTENT_RA: OrdThread.consistent L Ordering.acqrel e1_ra>>) \/
-       exists rels2 rels3 e_ra e2_ra e3_ra loc to val released ord,
-         (<<STEPS_RA: WThread.tau_steps L rels1 rels2 e1_ra e2_ra>>) /\
-         (<<CONS: Local.promise_consistent (Thread.local e2_ra)>>) /\
-         (<<STEP_RA: WThread.step L Ordering.acqrel Ordering.acqrel rels2 rels3 e_ra e2_ra e3_ra>>) /\
-         (<<READ: ThreadEvent.is_reading e_ra = Some (loc, to, val, released, ord)>>) /\
-         (<<RACE: RARaceW.ra_race L rels2 (Local.tview (Thread.local e2_ra)) loc to ord>>)).
+      (<<CONSISTENT_APF: OrdThread.consistent L Ordering.na Ordering.plain e1_apf>>) /\
+      (<<CONSISTENT_RA: OrdThread.consistent L Ordering.acqrel Ordering.acqrel e1_ra>>) \/
+      (exists rels2 e2_ra e st3,
+          (<<STEPS_RA: WThread.tau_steps L Ordering.acqrel Ordering.acqrel rels1 rels2 e1_ra e2_ra>>) /\
+          (<<CONS: Local.promise_consistent (Thread.local e2_ra)>>) /\
+          (<<STEP_RA: lang.(Language.step) e e2_ra.(Thread.state) st3>>) /\
+          (<<RACE: RARaceW.ra_race L rels2 (Local.tview (Thread.local e2_ra)) e>>)).
     Proof.
-      split.
-      { eapply JSim.sim_thread_consistent;
-          try eapply SIM1; try eapply WF1_PF; try eapply WF1_J.
-        inv CONSISTENT. des.
-        eapply Trace.consistent_thread_consistent; eauto. }
+      hexploit JSim.sim_thread_consistent;
+        try eapply SIM1; try eapply WF1_PF; try eapply WF1_J.
+      { inv CONSISTENT. des.
+        eapply Trace.consistent_thread_consistent; eauto.
+      }
+      intro CONSISTENT_J.
       exploit Memory.cap_exists; try apply WF1_PF. i. des.
       exploit Memory.cap_exists; try apply WF1_J. i. des.
+      exploit Memory.cap_exists; try apply WF1_APF. i. des.
       exploit Memory.cap_exists; try apply WF1_RA. i. des.
       exploit Memory.cap_closed; try eapply WF1_PF; eauto. i.
       exploit Memory.cap_closed; try eapply WF1_J; eauto. i.
+      exploit Memory.cap_closed; try eapply WF1_APF; eauto. i.
       exploit Memory.cap_closed; try eapply WF1_RA; eauto. i.
-      exploit Memory.max_concrete_timemap_exists; try eapply x0. i. des.
-      exploit Memory.max_concrete_timemap_exists; try eapply x1. i. des.
-      exploit Memory.max_concrete_timemap_exists; try eapply x2. i. des.
       exploit sim_thread_cap; eauto. i. des.
       inv CONSISTENT. des. exploit CONSISTENT; eauto. i. des.
-      - exploit sim_thread_steps; try exact STEPS; eauto.
-        { inv FAILURE; inv STEP. inv LOCAL. inv LOCAL0. ss. }
+      { (* failure *)
+        exploit sim_thread_steps; try exact STEPS; eauto.
+        { inv FAILURE; inv STEP; ss. inv LOCAL; ss; inv LOCAL0; ss. }
         i. des.
-        + exploit steps_pf_future; try exact STEPS; eauto. i. des.
+        - exploit steps_pf_future; try exact STEPS; eauto. i. des.
           exploit steps_j_future; try exact STEPS_J; eauto. i. des.
           exploit steps_ra_future; try eapply WThread.tau_steps_steps;
+            try exact STEPS_APF; eauto. i. des.
+          exploit steps_ra_future; try eapply WThread.tau_steps_steps;
             try exact STEPS_RA; eauto. i. des.
-          exploit sim_thread_step; try exact FAILURE; eauto; ss.
-          { inv FAILURE; inv STEP. inv LOCAL. inv LOCAL0. ss. }
+          exploit sim_thread_step; try exact FAILURE; eauto.
+          { inv FAILURE; inv STEP; ss. inv LOCAL; ss; inv LOCAL0; ss. }
+          { inv FAILURE; inv STEP; ss. inv LOCAL; ss; inv LOCAL0; ss. }
           i. des.
-          * left. ii. left.
-            exploit Memory.cap_inj; [exact CAP2|exact CAP1|..]; try apply WF1_RA. i. subst.
-            exploit Memory.max_concrete_timemap_inj; [exact SC_MAX|exact x5|]. i. subst.
-            inv EVENT_J; inv EVENT_RA.
-            exploit WThread.tau_steps_ord_tau_steps; try exact STEPS_RA. i.
-            inv STEP_RA. dup STEP. inv STEP0; [inv STEP1|].
-            unfold OrdThread.steps_failure. esplits; eauto.
-          * right.
-            exploit WThread.cap_plus_step_current_plus_step;
+          + left. splits; ss.
+            * ii. left.
+              exploit Memory.cap_inj; [exact CAP1|exact CAP3|..]; try apply WF1_APF. i. subst.
+              exploit WThread.tau_steps_ord_tau_steps; try exact STEPS_APF. i.
+              inv STEP_APF. destruct pf; cycle 1.
+              { inv STEP. inv STEP0. inv EVENT_APF; inv EVENT_J; ss. }
+              unfold OrdThread.steps_failure. esplits; eauto.
+              inv EVENT_APF; inv EVENT_J; ss.
+            * ii. left.
+              exploit Memory.cap_inj; [exact CAP2|exact CAP3|..]; try apply WF1_RA. i. subst.
+              exploit WThread.tau_steps_ord_tau_steps; try exact STEPS_RA. i.
+              inv STEP_RA. destruct pf; cycle 1.
+              { inv STEP. inv STEP0. inv EVENT_RA; inv EVENT_APF; inv EVENT_J; ss. }
+              unfold OrdThread.steps_failure. esplits; eauto.
+              inv EVENT_RA; inv EVENT_APF; inv EVENT_J; ss.
+          + right.
+            exploit WThread.cap_tau_steps_current_tau_steps;
               try exact STEPS_RA; eauto; try apply WF1_RA. i. des.
-            destruct e_ra; inv READ.
-            { inv EVENT. inv TO. esplits; eauto; ss.
-              - eapply local_map_promise_consistent; eauto.
-              - eapply local_map_ra_race; eauto. }
-            { inv EVENT. inv FROM. esplits; eauto; ss.
-              - eapply local_map_promise_consistent; eauto.
-              - eapply local_map_ra_race; eauto. }
-        + right.
-          exploit WThread.cap_plus_step_current_plus_step;
+            inv THREAD. ss.
+            hexploit local_map_promise_consistent; try eapply LOCAL; eauto. i.
+            esplits; eauto. s.
+            eapply local_map_ra_race; eauto.
+        - right.
+          exploit WThread.cap_tau_steps_current_tau_steps;
             try exact STEPS_RA; eauto; try apply WF1_RA. i. des.
-          destruct e_ra; inv READ.
-          { inv EVENT. inv TO. esplits; eauto; ss.
-            - eapply local_map_promise_consistent; eauto.
-            - eapply local_map_ra_race; eauto. }
-          { inv EVENT. inv FROM. esplits; eauto; ss.
-            - eapply local_map_promise_consistent; eauto.
-            - eapply local_map_ra_race; eauto. }
-      - exploit sim_thread_steps; try exact STEPS; eauto.
+          inv THREAD. ss.
+          hexploit local_map_promise_consistent; try eapply LOCAL; eauto. i.
+          esplits; eauto. s.
+          eapply local_map_ra_race; eauto.
+      }
+      { exploit sim_thread_steps; try exact STEPS; eauto.
         { ii. rewrite PROMISES in *. rewrite Memory.bot_get in *. ss. }
         i. des.
-        + left. ii. right.
-          exploit Memory.cap_inj; [exact CAP2|exact CAP1|..]; try apply WF1_RA. i. subst.
-          exploit Memory.max_concrete_timemap_inj; [exact SC_MAX|exact x5|]. i. subst.
-          exploit WThread.tau_steps_ord_tau_steps; try exact STEPS_RA. i.
-          esplits; eauto.
-          inv SIM2. inv SIM_JOINED.
-          apply inj_pair2 in H2. apply inj_pair2 in H3. subst. ss.
-          exploit JSim.sim_local_memory_bot; eauto. i.
-          inv SIM_RA. ss. subst. inv LOCAL0. congr.
-        + right.
-          exploit WThread.cap_plus_step_current_plus_step;
+        - left. splits; ss.
+          + ii. right.
+            exploit Memory.cap_inj; [exact CAP1|exact CAP3|..]; try apply WF1_APF. i. subst.
+            exploit WThread.tau_steps_ord_tau_steps; try exact STEPS_APF. i.
+            esplits; eauto.
+            inv SIM2. inv SIM_APF. rewrite LOCAL.
+            inv SIM_JOINED.
+            apply inj_pair2 in H2. apply inj_pair2 in H3. subst. ss.
+            exploit JSim.sim_local_memory_bot; eauto.
+          + ii. right.
+            exploit Memory.cap_inj; [exact CAP2|exact CAP3|..]; try apply WF1_RA. i. subst.
+            exploit WThread.tau_steps_ord_tau_steps; try exact STEPS_RA. i.
+            esplits; eauto.
+            inv SIM2. inv SIM_RA. inv LOCAL. rewrite PROMISES0.
+            inv SIM_APF. rewrite LOCAL.
+            inv SIM_JOINED.
+            apply inj_pair2 in H2. apply inj_pair2 in H3. subst. ss.
+            exploit JSim.sim_local_memory_bot; eauto.
+        - right.
+          exploit WThread.cap_tau_steps_current_tau_steps;
             try exact STEPS_RA; eauto; try apply WF1_RA. i. des.
-          destruct e_ra; inv READ.
-          { inv EVENT. inv TO. esplits; eauto; ss.
-            - eapply local_map_promise_consistent; eauto.
-            - eapply local_map_ra_race; eauto. }
-          { inv EVENT. inv FROM. esplits; eauto; ss.
-            - eapply local_map_promise_consistent; eauto.
-            - eapply local_map_ra_race; eauto. }
+          inv THREAD. ss.
+          hexploit local_map_promise_consistent; try eapply LOCAL; eauto. i.
+          esplits; eauto. s.
+          eapply local_map_ra_race; eauto.
+      }
     Qed.
   End PFtoRAThread.
 End PFtoRAThread.
